move to same file due to compspec problems

kalloc/kalloc.c
@@ -6,6 +6,7 @@
 
 //extern char end[]; // first address after kernel.
                    // defined by kernel.ld.
+                   
 
 struct run {
   struct run *next;
@@ -51,3 +52,165 @@ void *kalloc(void)
     kmem.freelist = r->next;
   return (void*)r; 
 }
+
+
+
+
+
+
+/// clients
+
+
+#define PGSIZE 4096 // bytes per page - original saved in risc.h
+#define PIPESIZE 512
+typedef unsigned int   uint;
+
+struct pipe {
+  char data[PIPESIZE];
+  uint nread;     // number of bytes read
+  uint nwrite;    // number of bytes written
+  int readopen;   // read fd is still open
+  int writeopen;  // write fd is still open
+};
+
+// verified
+
+// should return pa
+void *kfree_kalloc(void *pa) {
+  kfree(pa);
+  return kalloc();
+}
+
+// very simple - just to check if it can be used for a pipe..
+
+
+int kalloc_write_42(void) {
+
+  int *pa;
+  pa = 0;
+  pa = (int*)kalloc();           // cast to int pointer
+  if (pa) {
+    *pa = 42;
+    int X = *pa;
+    return X;
+  }
+  return 0;
+}
+
+
+int kalloc_write_42_kfree(void) {
+
+  int *pa;
+  pa = 0;
+  pa = (int*)kalloc();           // cast to int pointer
+  if (pa) {
+    *pa = 42;
+    int X = *pa;
+    kfree(pa);
+    return X;
+  }
+  return 0;
+}
+
+void kalloc_write_pipe()
+{
+  struct pipe *pi;
+
+  pi = 0;
+  pi = (struct pipe*)kalloc(); 
+  if(pi) {
+    pi->readopen = 1;
+    pi->writeopen = 1;
+    pi->nwrite = 0;
+    pi->nread = 0;
+  }
+}
+
+// working in progress
+
+// not added to client 1 yet -- it is in simple-kfree
+void freerange_while_loop(void *pa_start, void *pa_end) {  // admit on pointer
+  while ((char*)pa_start + PGSIZE <= (char*)pa_end) { 
+      kfree(pa_start);
+      pa_start = (char*)pa_start + PGSIZE;
+  }
+}
+
+// should return pa1
+void *client5(void *pa1, void *pa2) { // original 2
+  kfree(pa1);
+  kfree(pa2);
+  kalloc();
+  return kalloc();
+}
+
+
+// should return pa2
+void *client6(void *pa1, void *pa2) { // original 3
+  kfree(pa1);
+  kfree(pa2);
+  return kalloc();
+}
+
+void *client7(void *pa1, void *pa2) { // original 4
+  kfree_kalloc(pa1);
+  return kfree_kalloc(pa2);
+}
+
+void *client8(void *pa1, void *pa2) { // original 5
+  kfree(pa1);
+  kalloc();
+  kfree(pa2);
+  return kalloc();
+}
+
+
+void *client9(void *pa_start) { // original 6
+  int i = 0;
+  while (i < 2) {
+      kfree(pa_start);
+      pa_start = (char*)pa_start + PGSIZE;
+      i++;
+  }
+  return kalloc();
+}
+
+void *client10(void *pa_start, int n) { // original 7
+  int i = 0;
+  while (i < n) {
+      kfree(pa_start);
+      pa_start = (char*)pa_start + PGSIZE;
+      i++;
+  }
+  return kalloc();
+}
+
+void client11(void *pa_start, int n) { // original 8
+  int i = 0;
+  while (i < n) {
+      kfree(pa_start);
+      pa_start = (char*)pa_start + PGSIZE;
+      i++;
+  }
+}
+
+// this is basicly doing the same as client original 7
+void* client12(void *pa_start, int n) { // original 7
+  client11(pa_start, n);
+  return kalloc();
+}
+
+// this is allowed..
+void client13(void *pa_start) {
+  kfree(pa_start);
+  kfree(pa_start);
+}
+
+
+// working in progress.. simple version of pipealloc without allocating the files..
+
+
+
+
+
+
