kalloc/kalloc.h
@@ -1,2 +1,0 @@
-void*           kalloc(void);
-void            kfree(void *);
