kalloc/Verif_kalloc_kfree.v
@@ -1,7 +1,6 @@
 Require Import VST.floyd.proofauto.
 Require Import VC.ASI_kalloc.
 Require Import VC.kalloc.
-Require Import VC.clients.
 Require Import VC.kallocfun.
 Require Import VC.tactics.
 Require Import VC.Spec_kalloc.
@@ -9,12 +8,14 @@ Require Import VC.Spec_kalloc.
 (*#[export] Instance CompSpecs : compspecs. make_compspecs prog. Defined.
 Definition Vprog : varspecs. mk_varspecs prog. Defined.*)
 
-(*Local Open Scope logic.*)
+
 
 (*Require Import malloc.
 Require Import malloc_lemmas.
 Require Import malloc_sep.*)
 Require Import VC.kalloc_kfree_definitions.
+
+Local Open Scope logic.
 
 Lemma body_kfree: semax_body MF_Vprog MF_Gprog f_kfree (kfree_spec KF_APD t_run).
 Proof. start_function. Intros.
