kalloc/constantsfun.v
@@ -1,4 +1,0 @@
-(********************** functional model and lemmas for clients *************)
-Require Import VST.floyd.proofauto.
-
-Definition PGSIZE : Z := 4096.
