kalloc/tactics.v
@@ -3,3 +3,5 @@
 Require Import VST.floyd.proofauto.
 
 Ltac auto_contradict := try discriminate; try contradiction.
+
+Definition PGSIZE : Z := 4096.
